\documentclass[12pt, letterpaper, twoside]{article}
\usepackage[utf8]{inputenc}

\title{The differentiation game}
\author{Novoselov Alexander \thanks{funded by the 434 team}}
\date{November 2024}

\begin{document}

\maketitle


Gentlemen, it's a great pleasure to inform you that today we are differentiating
\[\frac{{({(0)}-{(length)})}+{({(size)}^{(0)})}}{{({(2)}*{(A)})}*{({({(curiosity)}-{(1)})}^{(1)})}}\]

Where 
\[A = {({(length)}-{(2)})}^{(2)}\]


There we begin...
\[\frac{d}{dlength}{(curiosity)}-{(1)} = {(0)}-{(0)}\]


Where 
\[\frac{d}{dlength}{({(curiosity)}-{(1)})}^{(1)} = {({(0)}-{(0)})}*{({(1)}*{({({(curiosity)}-{(1)})}^{({(1)}-{(1)})})})}\]


Where 
\[\frac{d}{dlength}{(length)}-{(2)} = {(1)}-{(0)}\]


Where 
\[\frac{d}{dlength}{({(length)}-{(2)})}^{(2)} = {({(1)}-{(0)})}*{({(2)}*{({({(length)}-{(2)})}^{({(2)}-{(1)})})})}\]


Where 
\[\frac{d}{dlength}{(2)}*{({({(length)}-{(2)})}^{(2)})} = {({(0)}*{({({(length)}-{(2)})}^{(2)})})}+{({(2)}*{({({(1)}-{(0)})}*{(B)})})}\]


Where 
\[B = {(2)}*{({({(length)}-{(2)})}^{({(2)}-{(1)})})}\]

\[\frac{d}{dlength}{({(2)}*{({({(length)}-{(2)})}^{(2)})})}*{({({(curiosity)}-{(1)})}^{(1)})} = {({({(C)}+{(D)})}*{({({(curiosity)}-{(1)})}^{(1)})})}+{({({(2)}*{(E)})}*{({({(0)}-{(0)})}*{(F)})})}\]


Where 
\[F = {(1)}*{({({(curiosity)}-{(1)})}^{({(1)}-{(1)})})}\]

\[E = {({(length)}-{(2)})}^{(2)}\]

\[D = {(2)}*{({({(1)}-{(0)})}*{({(2)}*{(G)})})}\]

\[G = {({(length)}-{(2)})}^{({(2)}-{(1)})}\]

\[C = {(0)}*{({({(length)}-{(2)})}^{(2)})}\]

\[\frac{d}{dlength}{(size)}^{(0)} = {(0)}*{({(0)}*{({(size)}^{({(0)}-{(1)})})})}\]


Where 
\[\frac{d}{dlength}{(0)}-{(length)} = {(0)}-{(1)}\]


Where 
\[\frac{d}{dlength}{({(0)}-{(length)})}+{({(size)}^{(0)})} = {({(0)}-{(1)})}+{({(0)}*{({(0)}*{(H)})})}\]


Where 
\[H = {(size)}^{({(0)}-{(1)})}\]

\[\frac{d}{dlength}\frac{{({(0)}-{(length)})}+{({(size)}^{(0)})}}{{({(2)}*{(I)})}*{({({(curiosity)}-{(1)})}^{(1)})}} = \frac{{({(J)}*{(K)})}-{({(L)}*{(M)})}}{{({(N)}*{(O)})}*{({(P)}*{(Q)})}}\]


Where 
\[Q = {({(curiosity)}-{(1)})}^{(1)}\]

\[P = {(2)}*{({({(length)}-{(2)})}^{(2)})}\]

\[O = {({(curiosity)}-{(1)})}^{(1)}\]

\[N = {(2)}*{({({(length)}-{(2)})}^{(2)})}\]

\[M = {({({(R)}+{(S)})}*{({({(curiosity)}-{(1)})}^{(1)})})}+{({({(2)}*{(T)})}*{({({(0)}-{(0)})}*{(U)})})}\]

\[U = {(1)}*{({({(curiosity)}-{(1)})}^{({(1)}-{(1)})})}\]

\[T = {({(length)}-{(2)})}^{(2)}\]

\[S = {(2)}*{({({(1)}-{(0)})}*{({(2)}*{(V)})})}\]

\[V = {({(length)}-{(2)})}^{({(2)}-{(1)})}\]

\[R = {(0)}*{({({(length)}-{(2)})}^{(2)})}\]

\[L = {({(0)}-{(length)})}+{({(size)}^{(0)})}\]

\[K = {({(2)}*{({({(length)}-{(2)})}^{(2)})})}*{({({(curiosity)}-{(1)})}^{(1)})}\]

\[J = {({(0)}-{(1)})}+{({(0)}*{({(0)}*{(W)})})}\]

\[W = {(size)}^{({(0)}-{(1)})}\]

\[I = {({(length)}-{(2)})}^{(2)}\]


Let's see if we can apply constant folding:

There we shall optimize
{(0)}-{(1)}
as -1

There we shall optimize
{(0)}-{(1)}
as -1

There we shall optimize
{(1)}-{(0)}
as 1

There we shall optimize
{(2)}-{(1)}
as 1

There we shall optimize
{(0)}-{(0)}
as 0

There we shall optimize
{(1)}-{(1)}
as 0

Now we will try removing neutral elements:

Let's see if we can apply constant folding:

There we shall optimize
{(-1)}+{(0)}
as -1

Now we will try removing neutral elements:

Let's see if we can apply constant folding:

Now we will try removing neutral elements:

Finally, after a long battle, we emerged victorious:
\[\frac{{({(-1)}*{(X)})}-{({({(0)}-{(length)})}*{(Y)})}}{{({(Z)}*{({(curiosity)}-{(1)})})}*{({(A)}*{({(curiosity)}-{(1)})})}}\]

Where 
\[A = {(2)}*{({({(length)}-{(2)})}^{(2)})}\]

\[Z = {(2)}*{({({(length)}-{(2)})}^{(2)})}\]

\[Y = {({({(2)}*{(B)})}*{({(curiosity)}-{(1)})})}+{(0)}\]

\[B = {(2)}*{({(length)}-{(2)})}\]

\[X = {({(2)}*{({({(length)}-{(2)})}^{(2)})})}*{({(curiosity)}-{(1)})}\]



\end{document}